theories/Monad/OptionMonad.v
@@ -1,6 +1,6 @@
 Require Import Monad.
 
-Instance Monad_option : Monad option :=
+Global Instance Monad_option : Monad option :=
 { ret  := @Some 
 ; bind := fun _ c1 _ c2 => match c1 with 
                              | None => None
@@ -8,23 +8,32 @@ Instance Monad_option : Monad option :=
                            end 
 }.
 
-Instance Zero_option : Zero option :=
+Global Instance Zero_option : Zero option :=
 { zero := @None }.
 
-Definition optionT (m : Type -> Type) : Type -> Type := 
-  fun x => m (option x).
+Section Trans.
+  Variable m : Type -> Type.
 
-Instance Monad_optionT m (M : Monad m) : Monad (optionT m) :=
-{ ret := fun _ x => @ret m M _ (Some x)
-; bind := fun _ c1 _ c2 =>
-  @bind _ M _ c1 _ (fun c1 =>
-    match c1 with
-      | None => @ret _ M _ None
-      | Some v => c2 v
-    end)
-}.
+  Definition optionT : Type -> Type := 
+    fun x => m (option x).
 
-Instance Zero_optionT m (M : Monad m) : Zero (optionT m) :=
-{ zero := fun _ => @ret _ M _ None }.
+  Variable M : Monad m.
 
+  Global Instance Monad_optionT : Monad optionT :=
+  { ret := fun _ x => @ret m M _ (Some x)
+  ; bind := fun _ c1 _ c2 =>
+    @bind _ M _ c1 _ (fun c1 =>
+      match c1 with
+        | None => @ret _ M _ None
+        | Some v => c2 v
+      end)
+  }.
+
+  Global Instance Zero_optionT : Zero optionT :=
+  { zero := fun _ => @ret _ M _ None }.
+
+  Global Instance MonadT_optionT : MonadT optionT m :=
+  { lift := fun _ c => bind c (fun x => ret (ret x))
+  }.
+End Trans.
 
