theories/Monad/ContMonad.v
@@ -21,23 +21,38 @@ Section ContType.
 
   Global Instance Cont_cont : Cont cont :=
   { callCC := fun _ _ f => mkCont (fun c => runCont (f (fun x => mkCont (fun _ => c x))) c)
-  }.  
+  }.
+
+  Definition mapCont (f : Ans -> Ans) {a} (c : cont a) : cont a :=
+    mkCont (fun x => f (runCont c x)).
+
+  Definition withCont {a b} (f : (b -> Ans) -> (a -> Ans)) (c : cont a) : cont b :=
+    mkCont (fun x => runCont c (f x)).
 
   Variable m : Type -> Type.
 
   Record contT (t : Type) : Type := mkContT
   { runContT : (t -> m Ans) -> m Ans }.
 
-  Global Instance Monad_contT (M : Monad m) : Monad contT :=
+  Global Instance Monad_contT : Monad contT :=
   { ret := fun _ x => mkContT (fun k => k x)
   ; bind := fun _ c1 _ c2 =>
     mkContT (fun c => 
       runContT c1 (fun a => runContT (c2 a) c))
   }.
 
-  Global Instance Cont_contT (M : Monad m) : Cont contT :=
+  Global Instance Cont_contT : Cont contT :=
   { callCC := fun _ _ f => mkContT (fun c => runContT (f (fun x => mkContT (fun _ => c x))) c)
   }.
 
+  Global Instance MonadT_contT (M : Monad m) : MonadT contT m :=
+  { lift := fun _ c => mkContT (bind c)
+  }.
+
+  Definition mapContT (f : m Ans -> m Ans) {a} (c : contT a) : contT a :=
+    mkContT (fun x => f (runContT c x)).
+
+  Definition withContT {a b} (f : (b -> m Ans) -> (a -> m Ans)) (c : contT a) : contT b :=
+    mkContT (fun x => runContT c (f x)).
 
 End ContType.
